Generalize increasing map to arbitrary values in map

src/high/increasing_map.v
@@ -8,82 +8,152 @@ relation [R] will always be reflexive, and hence this does not matter. The
 _knowledge_ that [R] is reflexive may not always be available however (since
 we may not know that [R] is in fact the encoding of some preorder, and hence
 this definition works best. *)
-Definition increasing_map (R : relation2 positive) (ss : gmap nat positive) :=
-  ∀ i j (s s' : positive),
+Definition increasing_map {A} (R : relation2 A) (ss : gmap nat A) :=
+  ∀ i j (s s' : A),
     i < j → (ss !! i = Some s) → (ss !! j = Some s') → R s s'.
 
-Lemma increasing_map_singleton R t s :
-  increasing_map R {[ t := s ]}.
-Proof. intros ????? ?%lookup_singleton_Some ?%lookup_singleton_Some. lia. Qed.
+Section increasing_map.
+  Context {A : Type}.
+  Implicit Types (s : A) (R : relation2 A).
 
-Lemma increasing_map_empty R : increasing_map R ∅.
-Proof. intros ????? [=]. Qed.
+  Lemma increasing_map_singleton R t s :
+    increasing_map R {[ t := s ]}.
+  Proof. intros ????? ?%lookup_singleton_Some ?%lookup_singleton_Some. lia. Qed.
 
-Lemma increasing_map_insert order m t_i s_i :
-  increasing_map order m →
-  (forall t (s : positive), m !! t = Some s → t < t_i → order s s_i) →
-  (forall t (s : positive), m !! t = Some s → t_i < t → order s_i s) →
-  increasing_map order (<[t_i := s_i]> m).
-Proof.
-  intros increasing before after.
-  intros t1 t2 s1 s2 lt.
-  destruct (decide (t_i = t1)) as [eq1|neq1];
-    destruct (decide (t_i = t2)) as [eq2|neq2];
-    subst; rewrite ?lookup_insert; rewrite ?lookup_insert_ne; try done.
-  - lia.
-  - intros [= ->] ?.
-    eapply after; done.
-  - intros ? [= ->].
-    eapply before; done.
-  - by apply increasing.
-Qed.
+  Lemma increasing_map_empty R : increasing_map R ∅.
+  Proof. intros ????? [=]. Qed.
 
-Lemma increasing_map_insert_after order `{!Transitive order} m t_i s_i t_t s_t :
-  increasing_map order m →
-  m !! t_i = Some s_i →
-  order s_i s_t →
-  t_i < t_t →
-  (forall t_c (s_c : positive),
-    m !! t_c = Some s_c → t_i < t_c → order s_t s_c ∧ order s_c s_t) →
-  increasing_map order (<[t_t := s_t]> m).
-Proof.
-  intros increasing look sLe tLe par.
-  intros t1 t2 s1 s2 lt.
-  destruct (decide (t_t = t1)) as [eq1|neq1];
-    destruct (decide (t_t = t2)) as [eq2|neq2].
-    (* subst; rewrite ?lookup_insert; try (rewrite lookup_insert_ne; last done). *)
-  - lia.
-  - subst.
-    rewrite lookup_insert.
-    rewrite lookup_insert_ne; last done.
-    intros [= ->] ?.
-    eapply par; [done | lia].
-  - rewrite <- eq2 in *.
-    rewrite lookup_insert_ne; last done.
-    rewrite lookup_insert.
-    intros look2 [= ->].
-    pose proof (Nat.lt_total t_i t1) as [lt2|[?|?]].
-    * eapply par; done.
-    * simplify_eq. done.
-    * etrans; last apply sLe.
-      eapply increasing; [| apply look2 | apply look].
-      lia.
-  - do 2 (rewrite lookup_insert_ne; last done).
-    by apply increasing.
-Qed.
+  Lemma increasing_map_insert R m t_i s_i :
+    increasing_map R m →
+    (forall t s, m !! t = Some s → t < t_i → R s s_i) →
+    (forall t s, m !! t = Some s → t_i < t → R s_i s) →
+    increasing_map R (<[t_i := s_i]> m).
+  Proof.
+    intros increasing before after.
+    intros t1 t2 s1 s2 lt.
+    destruct (decide (t_i = t1)) as [eq1|neq1];
+      destruct (decide (t_i = t2)) as [eq2|neq2];
+      subst; rewrite ?lookup_insert; rewrite ?lookup_insert_ne; try done.
+    - lia.
+    - intros [= ->] ?.
+      eapply after; done.
+    - intros ? [= ->].
+      eapply before; done.
+    - by apply increasing.
+  Qed.
 
-Lemma increasing_map_insert_last order `{!Transitive order} m t_l s_l t_t s_t :
-  increasing_map order m →
-  map_no_later m t_l →
-  t_l < t_t →
-  m !! t_l = Some s_l →
-  order s_l s_t →
-  increasing_map order (<[t_t := s_t]> m).
-Proof.
-  intros ? nolater ? ? ?.
-  eapply increasing_map_insert_after; eauto.
-  intros t b c lt.
-  unfold map_no_later in *.
-  specialize (nolater t lt).
-  congruence.
-Qed.
+  Lemma increasing_map_insert_after R `{!Transitive R} m t_i t_t s_i s_t :
+    increasing_map R m →
+    m !! t_i = Some s_i →
+    R s_i s_t →
+    t_i < t_t →
+    (forall t_c (s_c : A),
+      m !! t_c = Some s_c → t_i < t_c → R s_t s_c ∧ R s_c s_t) →
+    increasing_map R (<[t_t := s_t]> m).
+  Proof.
+    intros increasing look sLe tLe par.
+    intros t1 t2 s1 s2 lt.
+    destruct (decide (t_t = t1)) as [eq1|neq1];
+      destruct (decide (t_t = t2)) as [eq2|neq2].
+      (* subst; rewrite ?lookup_insert; try (rewrite lookup_insert_ne; last done). *)
+    - lia.
+    - subst.
+      rewrite lookup_insert.
+      rewrite lookup_insert_ne; last done.
+      intros [= ->] ?.
+      eapply par; [done | lia].
+    - rewrite <- eq2 in *.
+      rewrite lookup_insert_ne; last done.
+      rewrite lookup_insert.
+      intros look2 [= ->].
+      pose proof (Nat.lt_total t_i t1) as [lt2|[?|?]].
+      * eapply par; done.
+      * simplify_eq. done.
+      * etrans; last apply sLe.
+        eapply increasing; [| apply look2 | apply look].
+        lia.
+    - do 2 (rewrite lookup_insert_ne; last done).
+      by apply increasing.
+  Qed.
+
+  Lemma increasing_map_insert_last R `{!Transitive R} m t_l s_l t_t s :
+    increasing_map R m →
+    map_no_later m t_l →
+    t_l < t_t →
+    m !! t_l = Some s_l →
+    R s_l s →
+    increasing_map R (<[t_t := s]> m).
+  Proof.
+    intros ? nolater ? ? ?.
+    eapply increasing_map_insert_after; eauto.
+    intros t b c lt.
+    unfold map_no_later in *.
+    specialize (nolater t lt).
+    congruence.
+  Qed.
+
+End increasing_map.
+
+Definition increasing_list {A} (R : relation A) (ss : list A) :=
+  ∀ i j s s', i < j → (ss !! i = Some s) → (ss !! j = Some s') → R s s'.
+
+Section increasing_list.
+  Context {A : Type}.
+  Implicit Types (s : A) (R : relation2 A).
+
+  (* Context `{SqSubsetEq ST, !PreOrder (⊑@{ST})}. *)
+  (* Implicit Types (s : ST). *)
+
+  Lemma increasing_list_singleton R s : increasing_list R [s].
+  Proof. intros [|][|]?????; try naive_solver. lia. Qed.
+
+  Lemma lookup_snoc_Some (l : list A) x x2 i :
+    (l ++ [x]) !! i = Some x2 →
+    (l !! i = Some x2) ∨ (length l = i ∧ x = x2).
+  Proof.
+    intros [look|[? [??]%list_lookup_singleton_Some]]%lookup_app_Some.
+    - left. apply look.
+    - right. auto with lia.
+  Qed.
+
+  Lemma increasing_list_last_greatest R `{!PreOrder R} ss s i s' :
+    increasing_list R ss →
+    last ss = Some s →
+    ss !! i = Some s' →
+    R s' s.
+  Proof.
+    rewrite last_lookup.
+    unfold increasing_list.
+    intros incr lookLast look.
+    destruct (decide (i = pred (length ss))).
+    { simplify_eq. reflexivity. }
+    eapply incr; try done.
+    apply lookup_lt_Some in look.
+    lia.
+  Qed.
+
+  Lemma increasing_list_snoc `{!PreOrder R} xs xs__last (x : A) :
+    (last xs) = Some xs__last →
+    R xs__last x →
+    increasing_list R xs → increasing_list R (xs ++ [x]).
+  Proof.
+    intros last incl incr.
+    intros ?????.
+    intros [?|[??]]%lookup_snoc_Some; intros [look|[??]]%lookup_snoc_Some.
+    * eapply incr; done.
+    * simplify_eq.
+      etrans; last apply incl.
+      eapply increasing_list_last_greatest; done.
+    * apply lookup_lt_Some in look. lia.
+    * lia.
+  Qed.
+
+  (** A lemma that ties [increasing_map] and [increasing_list] together. *)
+  Lemma increasing_map_to_increasing_list R m lo hi l :
+    increasing_map R m → map_slice m lo hi l → increasing_list R l.
+  Proof.
+    intros incr sl.
+    intros ?? ?? lt look1 look2.
+  Admit. (* Prove this later if we need it. *)
+
+End increasing_list.
