src/high/locations.v
@@ -19,59 +19,6 @@ From self.high Require Export abstract_state resources protocol modalities post_
 From self.high.resources Require Export bumpers preorders auth_map_map abstract_history.
 From self.high.modalities Require Export no_buffer.
 
-Definition increasing_list `{SqSubsetEq ST} (ss : list ST) :=
-  ∀ i j s s', i < j → (ss !! i = Some s) → (ss !! j = Some s') → s ⊑ s'.
-
-Section increasing_list.
-  Context `{SqSubsetEq ST, !PreOrder (⊑@{ST})}.
-  Implicit Types (s : ST).
-
-  Lemma increasing_list_singleton s : increasing_list [s].
-  Proof. intros [|][|]?????; try naive_solver. Qed.
-
-  Lemma lookup_snoc_Some {A} (l : list A) x x2 i :
-    (l ++ [x]) !! i = Some x2 →
-    (l !! i = Some x2) ∨ (length l = i ∧ x = x2).
-  Proof.
-    intros [look|[? [??]%list_lookup_singleton_Some]]%lookup_app_Some.
-    - left. apply look.
-    - right. auto with lia.
-  Qed.
-
-  Lemma increasing_list_last_greatest ss s i s' :
-    increasing_list ss →
-    last ss = Some s →
-    ss !! i = Some s' →
-    s' ⊑ s.
-  Proof.
-    rewrite last_lookup.
-    rewrite /increasing_list.
-    intros incr lookLast look.
-    destruct (decide (i = pred (length ss))).
-    { simplify_eq. reflexivity. }
-    eapply incr; try done.
-    apply lookup_lt_Some in look.
-    lia.
-  Qed.
-
-  Lemma increasing_list_snoc xs xs__last (x : ST) :
-    (last xs) = Some xs__last →
-    xs__last ⊑ x →
-    increasing_list xs → increasing_list (xs ++ [x]).
-  Proof.
-    intros last incl incr.
-    intros ?????.
-    intros [?|[??]]%lookup_snoc_Some; intros [look|[??]]%lookup_snoc_Some.
-    * eapply incr; done.
-    * simplify_eq.
-      etrans; last apply incl.
-      eapply increasing_list_last_greatest; done.
-    * apply lookup_lt_Some in look. lia.
-    * lia.
-  Qed.
-
-End increasing_list.
-
 Section points_to_at.
   Context `{nvmFixedG Σ, hGD : nvmDeltaG Σ, AbstractState ST}.
 
